isabelle/QuiescentResult.thy
@@ -1,5 +1,5 @@
 theory QuiescentResult
-imports Semantics
+imports Semantics PositiveAccounts
 begin
 
 lemma reduceContractStepPayIsQuiescent :
@@ -26,68 +26,91 @@ lemma reduceContractStepPayIsQuiescent :
   apply simp
   by (smt ReduceStepResult.distinct(1) case_prod_unfold)
 
-lemma reduceContractStepIsQuiescent : "reduceContractStep env sta cont = NotReduced \<Longrightarrow> isQuiescent cont"
+lemma reduceOneIsSomeIfNotEmptyAndPositive : "accs \<noteq> [] \<Longrightarrow> allAccountsPositive accs \<Longrightarrow> refundOne accs \<noteq> None"
+  by (metis allAccountsPositiveMeansFirstIsPositive option.distinct(1) refundOne.cases refundOne.simps(1))
+
+lemma reduceContractStepIsQuiescent : "validAndPositive_state sta \<Longrightarrow>
+                                       reduceContractStep env sta cont = NotReduced \<Longrightarrow> isQuiescent cont sta"
   apply (cases cont)
-  apply auto[1]
+  apply (simp only:reduceContractStep.simps)
+  apply (cases "accounts sta")
+  using reduceContractStepPayIsQuiescent apply fastforce
+  apply (cases "refundOne (accounts sta)")
+  apply (simp add: reduceOneIsSomeIfNotEmptyAndPositive)
+  apply (simp add: case_prod_beta')
   using reduceContractStepPayIsQuiescent apply fastforce
   apply simp
   using isQuiescent.simps(2) apply blast
   by (metis ReduceStepResult.distinct(1) reduceContractStep.simps(5))
 
-lemma reductionLoopIsQuiescent_aux : "
-       (\<And>x11 x12 x13 x14 x xa.
-           reduceContractStep env state contract = Reduced x11 x12 x13 x14 \<Longrightarrow>
-           x = (if x11 = ReduceNoWarning then warnings else x11 # warnings) \<Longrightarrow>
-           xa = (case x12 of ReduceNoPayment \<Rightarrow> payments | ReduceWithPayment payment \<Rightarrow> payment # payments) \<Longrightarrow>
-           reductionLoop env x13 x14 x xa = ContractQuiescent nwa nef nsta ncon \<Longrightarrow> isQuiescent ncon) \<Longrightarrow>
-       reductionLoop env state contract warnings payments = ContractQuiescent nwa nef nsta ncon \<Longrightarrow> isQuiescent ncon"
+lemma reductionLoopIsQuiescent_aux :
+  "(\<And>x11 x12 x13 x14 x xa.
+     reduceContractStep env state contract = Reduced x11 x12 x13 x14 \<Longrightarrow>
+     x = (if x11 = ReduceNoWarning then warnings else x11 # warnings) \<Longrightarrow>
+     xa = (case x12 of ReduceNoPayment \<Rightarrow> payments | ReduceWithPayment payment \<Rightarrow> payment # payments) \<Longrightarrow>
+     validAndPositive_state x13 \<Longrightarrow> reductionLoop env x13 x14 x xa = ContractQuiescent nwa nef nsta ncon \<Longrightarrow> isQuiescent ncon nsta) \<Longrightarrow>
+   validAndPositive_state state \<Longrightarrow> reductionLoop env state contract warnings payments = ContractQuiescent nwa nef nsta ncon \<Longrightarrow> isQuiescent ncon nsta"
+  apply (simp only:reductionLoop.simps [of env state contract warnings payments])
   apply (cases "reduceContractStep env state contract")
-  apply simp
-  apply metis
-  by (simp_all add: reduceContractStepIsQuiescent)
+  apply (metis (no_types, lifting) ReduceStepResult.simps(8) reduceContractStep_preserves_validAndPositive_state)
+  apply (simp add: reduceContractStepIsQuiescent)
+  by simp
 
-lemma reductionLoopIsQuiescent : "reductionLoop env sta c wa ef = ContractQuiescent nwa nef nsta ncon \<Longrightarrow> isQuiescent ncon"
+lemma reductionLoopIsQuiescent : "validAndPositive_state sta \<Longrightarrow>
+                                  reductionLoop env sta c wa ef = ContractQuiescent nwa nef nsta ncon \<Longrightarrow> isQuiescent ncon nsta"
   apply (induction env sta c wa ef rule:reductionLoop.induct)
   using reductionLoopIsQuiescent_aux by blast
 
-theorem reduceContractUntilQuiecentIsQuiescent : "reduceContractUntilQuiescent env sta c = ContractQuiescent wa ef nsta ncon \<Longrightarrow> isQuiescent ncon"
-  apply (simp only: reduceContractUntilQuiescent.simps)
-  by (simp add: reductionLoopIsQuiescent)
+theorem reduceContractUntilQuiecentIsQuiescent : "validAndPositive_state sta \<Longrightarrow>
+                                                  reduceContractUntilQuiescent env sta c = ContractQuiescent wa ef nsta ncon \<Longrightarrow> isQuiescent ncon nsta"
+  by (simp only:reduceContractUntilQuiescent.simps reductionLoopIsQuiescent)
 
-lemma applyAllInputsLoopIsQuiescent_base : "applyAllLoop env fixSta cont [] wa ef = ApplyAllSuccess nwa nef nsta ncon \<Longrightarrow> isQuiescent ncon"
+lemma applyAllInputsLoopIsQuiescent_base : "validAndPositive_state fixSta \<Longrightarrow>
+                                            applyAllLoop env fixSta cont [] wa ef = ApplyAllSuccess nwa nef nsta ncon \<Longrightarrow> isQuiescent ncon nsta"
   apply (cases "reduceContractUntilQuiescent env fixSta cont")
-  apply (simp del:reduceContractUntilQuiescent.simps)
-  using reduceContractUntilQuiecentIsQuiescent apply blast
-  by simp
+  by (simp_all del:reduceContractUntilQuiescent.simps validAndPositive_state.simps add:reduceContractUntilQuiecentIsQuiescent)
 
-lemma applyAllInputsLoopIsQuiescent_loop : "(\<And>env fixSta cont wa ef. applyAllLoop env fixSta cont inps wa ef = ApplyAllSuccess nwa nef nsta ncon \<Longrightarrow> isQuiescent ncon) \<Longrightarrow>
-       applyAllLoop env fixSta cont (a # inps) wa ef = ApplyAllSuccess nwa nef nsta ncon \<Longrightarrow> isQuiescent ncon"
+lemma applyAllInputsLoopIsQuiescent_loop : "(\<And>env fixSta cont wa ef.
+           validAndPositive_state fixSta \<Longrightarrow> applyAllLoop env fixSta cont inps wa ef = ApplyAllSuccess nwa nef nsta ncon \<Longrightarrow> isQuiescent ncon nsta) \<Longrightarrow>
+       validAndPositive_state fixSta \<Longrightarrow> applyAllLoop env fixSta cont (a # inps) wa ef = ApplyAllSuccess nwa nef nsta ncon \<Longrightarrow> isQuiescent ncon nsta"
   apply (cases "reduceContractUntilQuiescent env fixSta cont")
   apply (unfold applyAllLoop.simps [of "env" "fixSta"])
-  apply (simp del:applyAllLoop.simps reduceContractUntilQuiescent.simps)
-  apply (metis (no_types, lifting) ApplyAllResult.distinct(1) ApplyResult.exhaust ApplyResult.simps(4) ApplyResult.simps(5))
-  by simp
+  apply (simp only:ReduceResult.case list.case)
+  oops
+  (* apply (metis (mono_tags, lifting) ApplyAllResult.distinct(1) ApplyResult.exhaust ApplyResult.simps(4) ApplyResult.simps(5) applyInput_preserves_preserves_validAndPositive_state reduceContractUntilQuiescent_preserves_validAndPositive_state)
+     by simp *)
 
-lemma applyAllInputsLoopIsQuiescent : "applyAllLoop env fixSta cont inps wa ef = ApplyAllSuccess nwa nef nsta ncon \<Longrightarrow> isQuiescent ncon"
+lemma applyAllInputsLoopIsQuiescent : "validAndPositive_state fixSta \<Longrightarrow>
+                                       applyAllLoop env fixSta cont inps wa ef = ApplyAllSuccess nwa nef nsta ncon \<Longrightarrow> isQuiescent ncon nsta"
   apply (induction inps arbitrary:env fixSta cont wa ef)
   apply (simp add: applyAllInputsLoopIsQuiescent_base)
-  using applyAllInputsLoopIsQuiescent_loop by blast
+  oops
+  (* using applyAllInputsLoopIsQuiescent_loop by blast *)
 
-lemma applyAllInputsIsQuiescent : "applyAllInputs env fixSta cont inps = ApplyAllSuccess warnings payments newState newCont \<Longrightarrow> isQuiescent newCont"
-  by (simp add: applyAllInputsLoopIsQuiescent)
+lemma applyAllInputsIsQuiescent : "validAndPositive_state fixSta \<Longrightarrow>
+                                   applyAllInputs env fixSta cont inps = ApplyAllSuccess warnings payments newState newCont \<Longrightarrow> isQuiescent newCont newState"
+  oops
+  (* by (simp add: applyAllInputsLoopIsQuiescent) *)
 
-lemma computeTransactionIsQuiescent_aux : "computeTransaction (Transaction \<lparr>interval = interva, inputs = inps\<rparr>) sta cont
-                                            = TransactionOutput \<lparr> txOutWarnings = nwa,
-                                                                  txOutPayments = nef,
-                                                                  txOutState = nsta,
-                                                                  txOutContract = ncont\<rparr> \<Longrightarrow>
+lemma computeTransactionIsQuiescent_aux : "validAndPositive_state sta \<Longrightarrow>
+                                           computeTransaction (Transaction \<lparr>interval = interva, inputs = inps\<rparr>) sta cont
+                                             = TransactionOutput \<lparr> txOutWarnings = nwa,
+                                                                   txOutPayments = nef,
+                                                                   txOutState = nsta,
+                                                                   txOutContract = ncont\<rparr> \<Longrightarrow>
        fixInterval (interval (Transaction \<lparr>interval = interva, inputs = inps\<rparr>)) sta = IntervalTrimmed x11 x12
-       \<Longrightarrow> isQuiescent ncont"
-  by (smt ApplyAllResult.exhaust ApplyAllResult.simps(10) ApplyAllResult.simps(8) ApplyAllResult.simps(9) IntervalResult.simps(5) TransactionOutput.distinct(1) TransactionOutput.inject(1) TransactionOutputRecord.select_convs(4) applyAllInputsIsQuiescent computeTransaction.simps)
+       \<Longrightarrow> isQuiescent ncont nsta"
+  apply (simp only:computeTransaction.simps)
+  oops
+  (* by (smt ApplyAllResult.exhaust ApplyAllResult.simps(10) ApplyAllResult.simps(8) ApplyAllResult.simps(9) IntervalResult.simps(5) TransactionOutput.distinct(1) TransactionOutput.inject(1) TransactionOutputRecord.ext_inject applyAllInputs.simps applyAllInputsLoopIsQuiescent fixInterval_preserves_preserves_validAndPositive_state) *)
 
-theorem computeTransactionIsQuiescent : "computeTransaction traIn sta cont = TransactionOutput traOut \<Longrightarrow> isQuiescent (txOutContract traOut)"
+theorem computeTransactionIsQuiescent : "validAndPositive_state sta \<Longrightarrow>
+                                         computeTransaction traIn sta cont = TransactionOutput traOut \<Longrightarrow>
+                                         isQuiescent (txOutContract traOut) (txOutState traOut)"
+
   apply (cases "traIn")
   apply (cases "traOut")
-  by (smt IntervalResult.exhaust IntervalResult.simps(6) Transaction.update_convs(3) TransactionOutput.distinct(1) TransactionOutputRecord.select_convs(4) computeTransaction.elims computeTransactionIsQuiescent_aux old.unit.exhaust)
+  oops
+  (* by (smt IntervalResult.exhaust IntervalResult.simps(6) Transaction.update_convs(3) TransactionOutput.distinct(1) TransactionOutputRecord.surjective computeTransaction.simps computeTransactionIsQuiescent_aux old.unit.exhaust) *)
 
 end
